add exam

VA/01 - Dafny/99-examenes/2021-paula/exercise1.dfy
@@ -10,55 +10,56 @@
 //1.Define a predicate oneBiggerOnRight that given an array v and a valid index i
 //on that array, determines if there exists an element on i's right that is smaller 
 //than v[i]
-predicate oneBiggerOnRight(a: array<int>, i: int)
-reads a
-requires 0 <= i < a.Length
+predicate oneBiggerOnRight(v:array<int>,i:int)
+reads v
+requires 0 <= i < v.Length
 {
-	exists k:nat :: i < k < a.Length && a[k] < a[i]
+	exists j :: i < j < v.Length && v[i] > v[j]
 }
-
 
 //2.Define a function countBiggerOnRight that given an array v and a valid index i
 //on that array, returns the number of elements in segment [i..v.Length] that meet 
 //the property oneBiggerOnRight previously defined
-function countBiggerOnRight(a: array<int>, i: int): (res:int)
-decreases a.Length - i
-reads a
-requires 0 <= i < a.Length
+function countBiggerOnRight(v:array<int>,i:int):int
+reads v
+requires 0 <= i < v.Length
+decreases v.Length - i
 {
-	if i == a.Length - 1 then 0
-	else if oneBiggerOnRight(a, i) then 1 + countBiggerOnRight(a, i+1)
-	else countBiggerOnRight(a, i + 1)
+	if i == v.Length-1 then 0
+	else 
+		if oneBiggerOnRight(v,i) then 1 + countBiggerOnRight(v,i+1)
+		else countBiggerOnRight(v,i+1)
 }
-
-
 
 //3.Using function countBiggerOnRight, specify a method
 //that receives an array v of distinct elements and returns  
 //the number of elements that have a smaller element on the right 
-method biggerOnRight(a: array<int>) returns (res: int)
-requires a.Length > 0
-ensures res == countBiggerOnRight(a, 0)
+method count(v:array<int>) returns (c:int)
+requires forall i,j :: 0 <= i < v.Length && 0 <= j < v.Length && i != j ==> v[i] != v[j]
+requires v.Length > 0
+ensures c == countBiggerOnRight(v,0)
 {
-	var min :int := a[a.Length - 1];
-	var idx: int := a.Length - 1;
-	res:=0;
-	while(idx > 0)
-	decreases idx
-	invariant 0 <= idx < a.Length
-	invariant forall k: nat :: idx <= k < a.Length ==> min <= a[k]
-	invariant exists k :: idx <= k < a.Length && a[k] == min
-	invariant res == countBiggerOnRight(a, idx)
+	var i := v.Length-1;
+	var min := v[v.Length-1];
+	c := 0;
 
+	while (i > 0)
+		decreases i
+		invariant 0 <= i < v.Length
+		invariant c >= 0
+		invariant forall j :: i <= j < v.Length ==> min <= v[j]
+		invariant exists j :: i <= j < v.Length && v[j] == min
+		invariant c == countBiggerOnRight(v,i)
 	{
-		if(a[idx-1] > min){res := res + 1;}
-		else {min := a[idx - 1];}
-		idx := idx - 1;
+		if v[i-1] > min {
+			c := c+1;
+		}
+		else { //v[i-1]<min
+			min := v[i-1];
+		}
+		i := i-1;
 	}
 }
 
-
-
 //4. Implement and verify an algorithm that solves this problem.
 //A linear time algorithm will be better valued.  
-
